\begin{align}
    p_{00} &= -C + \delta \left[p_{00}\Bigr(\tilde{V}_{11}-\tilde{V}_{01}\Bigr) + q_{00}\Bigr(\tilde{V}_{10}-\tilde{V}_{00}\Bigr)\right] \\
    p_{10} &= -C + \delta \left[p_{01}\Bigr(\tilde{V}_{11}-\tilde{V}_{01}\Bigr) + q_{01}\Bigr(\tilde{V}_{10}-\tilde{V}_{00}\Bigr)\right] \\
    p_{01} &= \delta \left[p_{10}\Bigr(\tilde{V}_{11}-\tilde{V}_{01}\Bigr) + q_{10}\Bigr(\tilde{V}_{10}-\tilde{V}_{00}\Bigr)\right] \\
    p_{11} &= \delta \left[p_{11}\Bigr(\tilde{V}_{11}-\tilde{V}_{01}\Bigr) + q_{11}\Bigr(\tilde{V}_{10}-\tilde{V}_{00}\Bigr)\right] \\
    \tilde{V}_{00} &= p_{00}\Bigr[C + \frac{p_{00}}{2} \Bigr] + p_{00}^2\tilde{V}_{11} + p_{00}\tilde{V}_{11}
\end{align}
